channel.v
@@ -1,0 +1,171 @@
+From iris.base_logic Require Export invariants.
+From iris.algebra Require Import auth frac agree gmap.
+From iris_io Require Export lang rules.
+From iris.proofmode Require Import tactics.
+From iris_io Require Import lang rules.
+From iris Require Import proofmode.tactics.
+From iris.program_logic Require Import weakestpre lifting.
+From iris.algebra Require Import agree frac.
+
+CoInductive interleaving {A} : Stream A → Stream A → Stream A → Prop :=
+  interL v μ1 μ2 μ : interleaving μ1 μ2 μ →
+                     interleaving {|Shead := v; Stail := μ1 |} μ2
+                                  {|Shead := v; Stail := μ |}
+| interR v μ1 μ2 μ : interleaving μ1 μ2 μ →
+                     interleaving μ1 {|Shead := v; Stail := μ2 |}
+                                  {|Shead := v; Stail := μ |}.
+
+Lemma interleaving_inh {A} (μ1 μ2 : Stream A) : (interleaving μ1 μ2) μ1.
+Proof.
+  revert μ1 μ2.
+  cofix.
+  destruct μ1.
+  by constructor.
+Qed.
+
+Fixpoint append_l_s {A} (l : list A) (s : Stream A) :=
+  match l with
+  | [] => s
+  | a :: l' => {|Shead := a; Stail := append_l_s l' s |}
+  end.
+
+Class ChannelIG Σ := channelIG {
+   stream_inG :> inG Σ (prodR (fracR) (agreeR (leibnizC (Stream val))));
+   streams_inG :> inG Σ (prodR (fracR) (agreeR (leibnizC ((Stream val) → Prop))))
+}.
+
+Fixpoint of_list (l : list val) :=
+  match l with
+    [] => InjLV Plang.UnitV
+  | v :: l' => InjRV (PairV v (of_list l'))
+  end.
+
+Section channels.
+
+  Context `{!ChannelIG Σ, !heapIG Σ}.
+
+  Definition own_stream γ q μ :=
+    own γ (q, to_agree μ : (agreeR (leibnizC (Stream val)))).
+
+  Definition own_streams γ q M :=
+    own γ (q, to_agree M : (agreeR (leibnizC ((Stream val) → Prop)))).
+
+  Definition channel_inv queue γs1 γs2 γR : iProp Σ :=
+        (∃ vs (μ1 μ2 : Stream val) M,
+            queue ↦ (of_list vs) ∗
+                  own_stream γs1 (1/2)%Qp μ1 ∗
+                  own_stream γs2 (1/2)%Qp μ2 ∗
+                  own_streams γR (1/2)%Qp M ∗
+                  ⌜∀ μ', interleaving μ1 μ2 μ' → M (append_l_s vs μ')⌝
+        )%I.
+
+  Definition sender queue μ :=
+    (∃ γs γs1 γs2 γR,
+        inv (nroot .@ "channel") (channel_inv queue γs1 γs2 γR) ∗
+            own_stream γs (1/2)%Qp μ ∗ ⌜γs = γs1 ∨ γs = γs2⌝)%I.
+
+  Definition receiver queue l μ :=
+    (∃ γs1 γs2 γR M, inv (nroot .@ "channel") (channel_inv queue γs1 γs2 γR)
+                         ∗ own_streams γR (1/2)%Qp M ∗ cpvar l M μ)%I.
+
+  Definition new_channel :=
+    Lam (Pair Create_Pr (Alloc (InjL Plang.Unit))).
+
+  Lemma wp_new_channel μ1 μ2 :
+    {{{True}}}
+      App new_channel Plang.Unit
+    {{{q l, RET (PairV (PrV l) (LocV q));
+       sender q μ1 ∗ sender q μ2 ∗
+              ∃ μ, ⌜interleaving μ1 μ2 μ⌝ ∗ receiver q l μ
+    }}}.
+  Proof.
+    iIntros (Φ) "_ HΦ".
+    iApply wp_pure_step_later; auto.
+    iNext. asimpl.
+    iApply (wp_bind (fill [PairLCtx _])); simpl.
+    iApply (wp_create_pr _ (interleaving μ1 μ2)); eauto using interleaving_inh.
+    iNext.
+    iIntros (l); iDestruct 1 as (μ) "Hμ".
+    iApply (wp_bind (fill [PairRCtx _])); simpl.
+    iApply wp_alloc; auto.
+    iNext. iIntros (q) "Hq".
+    iApply wp_value_fupd.
+    iMod (own_alloc (1%Qp, to_agree μ1 : (agreeR (leibnizC (Stream val)))))
+      as (γs1) "[Hμ11 Hμ12]";
+      first done.
+    iMod (own_alloc (1%Qp, to_agree μ2 : (agreeR (leibnizC (Stream val)))))
+      as (γs2) "[Hμ21 Hμ22]";
+      first done.
+    iMod (own_alloc (1%Qp, to_agree (interleaving μ1 μ2)
+                     : (agreeR (leibnizC (Stream val → Prop)))))
+      as (γR) "[HM1 HM2]";
+      first done.
+    iMod (inv_alloc (nroot .@ "channel") _ (channel_inv q γs1 γs2 γR)
+            with "[Hμ11 Hμ21 HM1 Hq]") as "#Hinv".
+    { iNext. unfold channel_inv.
+      iExists [], _, _, _; iFrame; auto. }
+    iModIntro.
+    iApply "HΦ".
+    iSplitL "Hμ12"; first by iExists _, _, _, _; iFrame; iFrame "#"; eauto.
+    iSplitL "Hμ22"; first by iExists _, _, _, _; iFrame; iFrame "#"; eauto.
+    iExists μ; iSplit; first by iApply cpvar_contains.
+    iExists _, _, _, _; iFrame "#"; iFrame.
+  Qed.
+
+  Definition Append :=
+    Lam
+      (Rec
+         (Case
+            (Var 1) (Var 3)
+            (InjR (Pair (Fst (Var 0)) (App (Var 1) (Snd (Var 0)))) ))
+      ).
+
+  Lemma wp_Append `{heapIG Σ} l l' :
+    WP (App (App Append (of_val (of_list l))) (of_val (of_list l')))
+       {{w, ⌜w = of_list (l' ++ l)⌝}}%I.
+  Proof.
+    iApply (wp_bind (fill [AppLCtx _])).
+    iApply wp_pure_step_later; auto.
+    iNext.
+    asimpl.
+    iApply wp_value. simpl.
+    iLöb as "IH" forall (l').
+                   iApply wp_pure_step_later; auto.
+                   iNext.
+                   asimpl.
+                   destruct l'.
+                   - simpl. iApply wp_pure_step_later; auto.
+                     iNext. asimpl. by iApply wp_value.
+                   - simpl. iApply wp_pure_step_later; auto.
+                     iNext. asimpl.
+                     iApply (wp_bind (fill [InjRCtx])).
+                     iApply (wp_bind (fill [PairLCtx _])).
+                     iApply wp_pure_step_later; auto.
+                     iNext; iApply wp_value. simpl.
+                     iApply (wp_bind (fill [PairRCtx _])).
+                     iApply (wp_bind (fill [AppRCtx (RecV _)])).
+                     iApply wp_pure_step_later; auto.
+                     iNext; iApply wp_value. simpl.
+                     iApply wp_wand_r; iSplitR.
+                     { iApply "IH". }
+                     iIntros (w) "%"; subst; simpl.
+                       by do 2 iApply wp_value.
+  Qed.
+
+  Definition send :=
+    Lam
+      (Rec
+         (LetIn (Load (Snd (Var 2)))
+                (If
+                   (CAS (Snd (Var 3)) (Var 0) (App (App Append (Var 2)) (Var 3)))
+                   (Plang.Unit)
+                   (App (Var 1) (Var 2))
+                )
+         )
+      ).
+
+
+End channels.
+
+
+
